Start proof

types.v
@@ -2,105 +2,267 @@ Require Import Coq.ZArith.ZArith.
 Require Import Coq.Lists.List.
 
 
-(** These two definitions specify the _abstract syntax_ of
-    arithmetic and boolean expressions. *)
-
 Module Exp.
+
+Inductive mem_loc : Type :=
+| MemLoc : nat -> mem_loc.
+
+Definition mem_loc_to_nat (loc : mem_loc) : nat :=
+match loc with
+  | MemLoc n => n
+end.
+
+
+Inductive ref_type : Type :=
+| RefMut : mem_loc -> ref_type  
+| RefImm : mem_loc -> ref_type.
+
+Definition ref_to_mem_loc (ref : ref_type) : mem_loc :=
+match ref with
+| RefMut loc => loc
+| RefImm loc => loc
+end.
+
 Inductive value : Type :=
-  | VUnit : value
-  | VInt : Z -> value
-  | VRefMut : Z -> value
-  | VRefImmMut : Z -> value.
+| VUnit : value
+| VInt : Z -> value
+| VRefMut : ref_type -> value
+| VRefImmMut : ref_type -> value.
+
+Inductive var : Type := 
+| Var : nat -> var. 
+
+Definition var_to_nat (v : var) : nat :=
+match v with
+  | Var n => n
+end.
 
 Inductive expression : Type :=
-  | Evalue: value -> expression                   
-  | EVar : Z -> expression                            
-  | EAssign : Z -> expression -> expression        
-  | EMutBorrow : Z -> expression             
-  | EImmBorrow : Z -> expression             
-  | EDeref : expression -> expression                
-  | ELet : Z -> expression -> expression -> expression   
-  | ESequence : expression -> expression -> expression.          
+| EValue: value -> expression                   
+| EVar : var -> expression                            
+| EAssign : mem_loc -> expression -> expression        
+| EMutBorrow : mem_loc -> expression             
+| EImmBorrow : mem_loc -> expression             
+| EDeref : expression -> expression                
+| ELet : var -> expression -> expression -> expression
+| EMut : var -> expression -> expression
+| ESequence : expression -> expression -> expression.          
 
 
 Inductive ownership : Type :=
 | Own : value -> ownership 
-| BorrowMut : nat -> ownership               
-| BorrowImm : list nat -> ownership. 
+| BorrowMut : mem_loc -> ownership               
+| BorrowImm : list mem_loc -> ownership
+| OwnMut : value -> ownership.
 
-Definition memory_state := nat -> option ownership.
+Definition memory_state := mem_loc -> option ownership.
 
 Definition lifetime_state := nat -> nat.
 
 Inductive borrow_state : Type :=
-| MutBorrowed : nat -> borrow_state
-| ImmBorrowed : list nat -> borrow_state.
+| MutBorrowed : mem_loc -> borrow_state
+| ImmBorrowed : list mem_loc -> borrow_state.
 
-Definition update_memory (h : memory_state) (loc : nat) (v : option ownership) : memory_state :=
-  fun l => if l =? loc then v else h l.
+Definition update_memory (m : memory_state) (loc : mem_loc) (v : option ownership) : memory_state :=
+fun l => 
+  if Nat.eqb (mem_loc_to_nat l) (mem_loc_to_nat loc) then v 
+  else m l.
 
 
 Fixpoint eval (m : memory_state) (e : expression) : option (memory_state * value) :=
-  match e with
-  | EVal v => Some (h, v)
-  | EAdd e1 e2 =>
-      match eval h e1, eval h e2 with
-      | Some (h1, VInt v1), Some (h2, VInt v2) => Some (h2, VInt (v1 + v2))
-      | _, _ => None
+match e with
+  | EValue v => Some (m, v)
+  | EVar x =>
+      match m (MemLoc (var_to_nat x)) with
+        | Some (Own v) => Some (m, v)
+        | Some (OwnMut v) => Some (m, v)
+        | _ => None
       end
-  | ESub e1 e2 =>
-      match eval h e1, eval h e2 with
-      | Some (h1, VInt v1), Some (h2, VInt v2) => Some (h2, VInt (v1 - v2))
-      | _, _ => None
-      end
-  | EMul e1 e2 =>
-      match eval h e1, eval h e2 with
-      | Some (h1, VInt v1), Some (h2, VInt v2) => Some (h2, VInt (v1 * v2))
-      | _, _ => None
-      end
-  | EMutBorrow x =>
-      match h x with
-      | Some (Own v) => Some (update_heap h x (Some (BorrowMut x)), VRefMut x)
+  | EAssign loc e' =>
+    match eval m e' with
+      | Some (m', v) =>
+          match m loc with
+          | Some (OwnMut _) =>
+              Some (update_memory m' loc (Some (OwnMut v)), v)
+          | _ => None
+          end
+      | _ => None
+    end
+  | EMut loc e' =>
+    match m (MemLoc (var_to_nat loc)) with
+    | Some _ => None (* Fail if loc is already in use *)
+    | None =>
+        match eval m e' with
+        | Some (m', v) =>
+            match v with
+            | VInt _ => Some (update_memory m' (MemLoc (var_to_nat loc)) (Some (OwnMut v)), VUnit)
+            | _ => None (* Invalid value for mutable binding *)
+            end
+        | _ => None
+        end
+    end
+  | EMutBorrow loc =>
+      match m loc with
+      | Some (Own v) =>
+          Some (update_memory m loc (Some (BorrowMut loc)), VRefMut (RefMut loc))
       | _ => None
       end
-  | EImmBorrow x =>
-      match h x with
-      | Some (Own v) => Some (update_heap h x (Some (BorrowImm [x])), VRefImm x)
+  | EImmBorrow loc =>
+      match m loc with
+      | Some (Own v) =>
+          Some (update_memory m loc (Some (BorrowImm (loc :: nil))), VRefImmMut (RefImm loc))
+      | Some (BorrowImm l) => 
+          Some (update_memory m loc (Some (BorrowImm (loc :: l))), VRefImmMut (RefImm loc))
+      | _ => None 
+      end
+  | EDeref e' =>
+      match eval m e' with
+        | Some (m', VRefMut loc) =>
+            match m (ref_to_mem_loc loc) with
+              | Some (OwnMut v) => Some (m', v)
+              | _ => None
+              end
+        | Some (m', VRefImmMut loc) =>
+            match m (ref_to_mem_loc loc) with
+              | Some (Own v) => Some (m', v) 
+              | _ => None 
+            end
+        | _ => None 
+      end
+  | ELet x e1 e2 =>
+      match eval m e1 with
+      | Some (m', v) =>
+          let new_m := update_memory m' (MemLoc (var_to_nat x)) (Some (Own v)) in
+          eval new_m e2
       | _ => None
       end
-  | EDeref e1 =>
-      match eval h e1 with
-      | Some (h1, VRefMut x) => match h x with Some (Own v) => Some (h1, v) | _ => None end
-      | Some (h1, VRefImm x) => match h x with Some (Own v) => Some (h1, v) | _ => None end
+  | ESequence e1 e2 =>
+      match eval m e1 with
+      | Some (m', _) => eval m' e2 
       | _ => None
       end
-  | _ => None 
-  end.
+end.
 
 
-Inductive borrow_valid : memory_state -> nat -> borrow_state -> Prop :=
-  | BorrowMutValid : forall h x,
-      h x = Some (BorrowMut x) ->
-      borrow_valid h x (MutBorrowed x)
-  | BorrowImmValid : forall h x l,
-      h x = Some (BorrowImm l) ->
-      Forall (fun r => h r = Some (BorrowImm l)) l ->
-      borrow_valid h x (ImmBorrowed l).
+Inductive borrow_valid : memory_state -> mem_loc -> borrow_state -> Prop :=
+  | BorrowMutValid : forall m loc,
+      m loc = Some (BorrowMut loc) ->
+      borrow_valid m loc (MutBorrowed loc)
+  | BorrowImmValid : forall m loc bs,
+      m loc = Some (BorrowImm bs) ->
+      Forall (fun r => m r = Some (BorrowImm bs)) bs ->
+      borrow_valid m loc (ImmBorrowed bs).
 
 
 Inductive has_type : lifetime_state -> memory_state -> expression -> ref_type -> Prop :=
-| TVal : forall l h v,
-    has_type l h (EVal v) (RefImm 0) (* Values are immutable *)
-| TAdd : forall l h e1 e2,
-    has_type l h e1 (RefImm 0) -> (* Operands must be integers *)
-    has_type l h e2 (RefImm 0) ->
-    has_type l h (EAdd e1 e2) (RefImm 0)
-| TMutBorrow : forall l h x t,
-    has_type l h (EVar x) (RefMut t) ->
-    has_type l h (EMutBorrow x) (RefMut t)
-| TImmBorrow : forall l h x t,
-    has_type l h (EVar x) (RefImm t) ->
-    has_type l h (EImmBorrow x) (RefImm t).
+| TValInt : forall (l : lifetime_state) (m : memory_state) (z : Z),
+    has_type l m (EValue (VInt z)) (RefImm (MemLoc 0)) (* Integer literals *)
+
+| TValRefMut : forall (l : lifetime_state) (m : memory_state) (loc : mem_loc),
+    has_type l m (EValue (VRefMut (RefMut loc))) (RefMut loc) (* Mutable references *)
+
+| TValRefImm : forall (l : lifetime_state) (m : memory_state) (loc : mem_loc),
+    has_type l m (EValue (VRefImmMut (RefImm loc))) (RefImm loc) (* Immutable references *)
+
+| TValUnit : forall (l : lifetime_state) (m : memory_state),
+    has_type l m (EValue VUnit) (RefImm (MemLoc 0)) (* Unit type *)
+| TVar : forall (l : lifetime_state) (m : memory_state) (x : var) (r : ref_type),
+    (* Variable typing requires ownership to be convertible to a reference type *)
+    match m (MemLoc (var_to_nat x)) with
+    | Some (Own _) => r = RefImm (MemLoc (var_to_nat x))
+    | Some (BorrowMut loc) => r = RefMut loc
+    | Some (BorrowImm locs) => r = RefImm (MemLoc (var_to_nat x))
+    | _ => False (* Invalid case *)
+    end ->
+    has_type l m (EVar x) r
+| TMutBorrow : forall l m x t,
+    (* Mutable borrow is valid if the variable has a mutable type *)
+    has_type l m (EVar x) (RefMut t) ->
+    has_type l m (EMutBorrow (MemLoc (var_to_nat x))) (RefMut t)
+
+| TImmBorrow : forall (l : lifetime_state) (m : memory_state) (x : var) (loc : mem_loc),
+    (* Immutable borrow is valid if the variable has an immutable type *)
+    has_type l m (EVar x) (RefImm loc)->
+    has_type l m (EImmBorrow (MemLoc (var_to_nat x))) (RefImm loc)
+
+| TMut : forall (l : lifetime_state) (m : memory_state) (x : var) (e : expression) (r : ref_type),
+    (* Mutability ensures the binding is treated as mutable *)
+    has_type l m e r ->
+    has_type l m (EMut x e) r.
+
+Theorem type_safety : 
+forall (l : lifetime_state) (m : memory_state) (e : expression) (r : ref_type) (m' : memory_state) (v : value),
+ has_type l m e r ->             
+  (exists m' v, eval m e = Some (m', v)) \/ eval m e = None.
+Proof.
+  (* intros l m e r Htype. *)
+  intros l m e r m' v Htype.
+  generalize dependent v.
+  induction e.
+  - left. exists m, v. simpl. reflexivity.
+  - simpl. destruct (m (MemLoc (var_to_nat v))).
+    + destruct o.
+      * left. exists m, v0. reflexivity.
+      * right. reflexivity.
+      * right. reflexivity.
+      * left. exists m, v0. reflexivity.
+    + right. reflexivity.
+  - intros v. inversion Htype.
+  - simpl. inversion Htype. subst r. rewrite <- H in *.  destruct (m (MemLoc (var_to_nat x))) eqn:Hlookup.
+    + destruct o.
+      * left. 
+      exists (update_memory m (MemLoc (var_to_nat x)) (Some (BorrowMut (MemLoc (var_to_nat x))))),
+      (VRefMut (RefMut (MemLoc (var_to_nat x)))).
+reflexivity.
+      * right. reflexivity.
+      * right. reflexivity.
+      * right. reflexivity.
+    + right. reflexivity.
+  - simpl. inversion Htype. subst r. rewrite <- H in *. destruct (m (MemLoc (var_to_nat x))).
+    + destruct o.
+      * left. exists (update_memory m (MemLoc (var_to_nat x)) (Some (BorrowImm (MemLoc (var_to_nat x) :: nil)))).
+      exists (VRefImmMut (RefImm (MemLoc (var_to_nat x)))). reflexivity.
+      * right. reflexivity.
+      * left. exists (update_memory m (MemLoc (var_to_nat x)) (Some (BorrowImm (MemLoc (var_to_nat x) :: l1)))).
+      exists (VRefImmMut (RefImm (MemLoc (var_to_nat x)))). reflexivity.
+      * right. reflexivity.
+    + right. reflexivity.
+  - inversion Htype.
+  - inversion Htype.
+  - intros. simpl. inversion Htype.
+    destruct (IHe H4) as [[m'' [v' Heval]] | Heval].
+    + auto.
+    + simpl.
+      destruct (m (MemLoc (var_to_nat v))) eqn:Hlookup.
+      * (* Case: m (MemLoc (var_to_nat v)) = Some _ *)
+        right. reflexivity. (* Borrow fails because the location is already in use *)
+      * (* Case: m (MemLoc (var_to_nat v)) = None *)
+        destruct v'.
+        -- (* Case: v' = VInt z *)
+          exists (update_memory m'' (MemLoc (var_to_nat v)) (Some (OwnMut (VInt 0)))).
+          exists VUnit.
+          reflexivity.
+        * (* Case: v' = VRefMut loc *)
+          right. reflexivity. (* Borrow fails for invalid value *)
+        * (* Case: v' = VRefImm loc *)
+          right. reflexivity. (* Borrow fails for invalid value *)
+        * (* Case: v' = VUnit *)
+          right. reflexivity. (* Borrow fails for invalid value *)
+        reflexivity.
+    
+    
+  
+  - 
+Admitted.
+
+Theorem borrow_safety : 
+forall (l : lifetime_state) (m : memory_state) (e: expression) (r : ref_type) (m' : memory_state) (v : value) (loc : mem_loc) (bs : borrow_state),
+  has_type l m e r ->         
+  borrow_valid m loc bs ->                
+  eval m e = Some (m', v) -> 
+  borrow_valid m' loc bs.
+Proof.
+Admitted.
 
 
 End Exp.
